doc/tutorial/code/exercises/ex10-shift.fst
@@ -1,0 +1,42 @@
+module Ex10b
+open Heap
+open ST
+
+type point =
+  | Point : x:ref int -> y:ref int{y<>x} -> point
+
+val new_point: x:int -> y:int -> ST point
+  (requires (fun h -> True))
+  (ensures (fun h0 p h1 ->
+                modifies Set.empty h0 h1
+                /\ fresh (Point.x p ^+^ Point.y p) h0 h1
+                /\ Heap.sel h1 (Point.x p) = x
+                /\ Heap.sel h1 (Point.y p) = y))
+let new_point x y =
+  let x = ref x in
+  let y = ref y in
+  Point x y
+
+let shift p =
+  Point.x p := !(Point.x p) + 1;
+  Point.y p := 17
+
+val shift_p1: p1:point
+           -> p2:point{   Point.x p2 <> Point.x p1
+                       /\ Point.y p2 <> Point.x p1 }
+           -> ST unit
+    (requires (fun h -> Heap.contains h (Point.x p2)
+                    /\  Heap.contains h (Point.y p2)))
+    (ensures (fun h0 _ h1 -> modifies (only (Point.x p1)) h0 h1))
+let shift_p1 p1 p2 =
+    let p2_0 = !(Point.x p2), !(Point.y p2)  in //p2 is initially p2_0
+    shift p1;
+    let p2_1 = !(Point.x p2), !(Point.y p2) in
+    assert (p2_0 = p2_1)                        //p2 is unchanged
+
+val test: unit -> St unit
+let test () =
+  let x = new_point 0 0 in
+  let y = new_point 0 1 in
+  (*shift_p1 x x;*)
+  shift_p1 x y
